proved the lemma chanacterixing Sine

icreate.v
@@ -2067,13 +2067,162 @@ Proof.
   apply DerivativerotateOriginTowards2; eauto with ICR.
 Qed.
 
+Hint Rewrite CFCosAp CFSineAp IContRPlusAp IContRMultAp IContRMinusAp : IContRApDown.
+Hint Unfold Negate_instance_TContR : TContRMC.
+
+
+(* remove *)
+Lemma IContRInvAp : ∀ (F: TContR) t,
+  {[--] F} t [=] [--] ({F} t).
+Proof.
+  intros. simpl.
+  reflexivity.
+Qed.
+Lemma IContRConstAp : ∀ (c: IR) t,
+  {ConstTContR c} t [=] c.
+Proof.
+  intros. simpl.
+  reflexivity.
+Qed.
+
+Hint Rewrite IContRInvAp IContRConstAp : IContRApDown.
+Hint Unfold Mult_instance_IR Zero_Instace_IR_better : IRMC.
+
+Instance Pi_Instance_IR: RealNumberPi ℝ :=
+ Pi.
+
+Hint Rewrite cg_zero_inv cg_inv_inv : CoRN.
+
+Lemma Sin_nonpos
+     : ∀ θ : ℝ, -π ≤ θ ≤ 0 -> Sin θ ≤ 0.
+Proof.
+  intros ? Hd.
+  apply inv_cancel_leEq.
+  autounfold with IRMC.
+  rewrite inj_Q_Zero.
+  autorewrite with CoRN.
+  rewrite <- Sin_inv.
+  repnd.
+  apply inv_resp_leEq in Hdr.
+  apply inv_resp_leEq in Hdl.
+  autounfold with IRMC in Hdl, Hdr.
+  rewrite inj_Q_Zero in Hdr.
+  autorewrite with CoRN in Hdr, Hdl.
+  apply Sin_nonneg; assumption.
+Qed.
+
+
+  
+
+Lemma AbsIRSine : ∀ θ, 
+  -π ≤ θ ≤ π
+  -> AbsIR (Sin θ) = Sin (AbsIR θ).
+Proof.
+  intros ? Hb.
+  pose proof (leEq_or_leEq _ θ [0]) as Hd.
+  apply not_ap_imp_eq.
+  intro Hc.
+  apply Hd.
+  clear Hd. intro Hd.
+  apply ap_tight in Hc;[contradiction|].
+  repnd.
+  destruct Hd as [c|].
+- unfold CanonicalNotations.norm, NormSpace_instance_IR. 
+  symmetry. rewrite AbsIR_eq_inv_x; [|assumption].
+  rewrite Sin_inv.
+  rewrite AbsIR_eq_inv_x; [reflexivity|].
+  rewrite <- inj_Q_Zero.
+  rewrite <- inj_Q_Zero in c.
+  apply Sin_nonpos; split; try assumption.
+- unfold CanonicalNotations.norm, NormSpace_instance_IR. 
+  symmetry. rewrite AbsIR_eq_x; [|assumption].
+  rewrite AbsIR_eq_x; [reflexivity|].
+  apply Sin_nonneg; assumption.
+Qed.
+
+(* consider changing types of [θErrTrnsl]
+    and [θErrTurn] to [Qpos]*)
+Variable ThetaErrLe90 :
+   θErrTrnsl + θErrTurn ≤  ('½) * π.
+
+Lemma PiBy2NoMC :
+   ('½) * π = Pi [/]TwoNZ.
+Proof.
+  apply (injective IRasCR).
+  rewrite <- CRPiBy2Correct.
+  unfold mult, Mult_instance_IR.
+  autorewrite with IRtoCR.
+  unfold cast, Cart_CR_IR.
+  rewrite CRasIRasCR_id.
+  pose proof (@rings.mult_comm CR _ _ _ _ _ _ ) as Hc.
+  unfold Commutative in Hc.
+  unfold mult in Hc.
+  rewrite Hc. reflexivity.
+Qed.
+
+Lemma ThetaErrLe90IR :
+   θErrTrnsl + θErrTurn ≤ Pi [/]TwoNZ.
+Proof.
+  rewrite <- PiBy2NoMC.
+  assumption.
+Qed.
+
+Hint Resolve pos_Pi : CoRN.
+Lemma ThetaErrLe1180 : 
+  θErrTrnsl + θErrTurn ≤  π.
+Proof.
+  rewrite PiBy2NoMC in ThetaErrLe90.
+  eapply leEq_transitive;[apply ThetaErrLe90 |].
+  apply nonneg_div_two'.
+  eauto using less_leEq, pos_Pi.
+Qed.
+
+Lemma PiBy2Ge0 : [0][<=]Pi [/]TwoNZ.
+Proof.
+  apply nonneg_div_two.
+  eauto using less_leEq, pos_Pi.
+Qed.
+  
+Lemma MinusPiBy2Le0 : [--](Pi [/]TwoNZ)[<=] [0].
+Proof.
+  apply inv_cancel_leEq.
+  autorewrite with CoRN.
+  apply PiBy2Ge0.
+Qed.
+
+Definition transErrTrans
+:= (rad (motorPrec {| rad := QposAsQ speed; θ := 0 |})).
+
+Hint Resolve PiBy2Ge0 MinusPiBy2Le0 AbsIR_nonneg: CoRN.
 (** prepping for [TDerivativeAbsQ] *)
 Lemma YDerivEv2To3 : ∀ (t:QTime), 
   let t3 : QTime := MotorEventsNthTime 3 (decAuto (3<4)%nat I) in
   let t2 : QTime := MotorEventsNthTime 2 (decAuto (2<4)%nat I) in
   t2 ≤ t ≤ t3 
-  → AbsIR ({YDerivRot} t) ≤  (Sin (θErrTrnsl + θErrTurn)) * speed.
+  → AbsIR ({YDerivRot} t) 
+      ≤   (Sin (θErrTrnsl + θErrTurn)) * (speed + transErrTrans)%Q.
+Proof.
+  intros ? ? ? Hb.
+  unfold YDerivRot.
+  autounfold with IRMC TContRMC.
+  fold (theta icreate[-](ConstTContR optimalTurnAngle)).
+  autorewrite with IContRApDown.
+  rewrite AbsIR_resp_mult.
+  rewrite mult_commut_unfolded.
+  apply mult_resp_leEq_both; try apply 
+    AbsIR_nonneg;[|].
+- apply ThetaEv2To3_3 in Hb.
+  rewrite  AbsIRSine;
+    [| apply AbsIR_imp_AbsSmall;
+       eapply leEq_transitive;[apply Hb|apply ThetaErrLe1180]].
+  apply TrigMon.Sin_resp_leEq; [| | assumption].
+  + info_eauto using leEq_transitive, 
+      MinusPiBy2Le0,AbsIR_nonneg.
+  + apply ThetaErrLe90IR.
+- admit.
 Abort.
+
+
 
   
 
